

1 Propositional Logic

1.1 Semantics

Definition 1.1 (Interpretation). An *interpretation* I is a function that maps each propositional variable to either true or false.

$$I : \{p_1 \mapsto \text{true} \vee \text{false}, p_2 \mapsto \text{true} \vee \text{false}, \dots, p_n \mapsto \text{true} \vee \text{false}\}$$

1.2 Syntax

Rule	$I \models \cdot$	$I \not\models \cdot$
Neg	$\frac{I \models \neg F}{I \not\models F}$	$\frac{I \not\models \neg F}{I \models F}$
Conj	$\frac{I \models F_1 \wedge F_2}{I \models F_1 \quad I \models F_2}$	$\frac{I \not\models F_1 \wedge F_2}{I \not\models F_1 \mid I \not\models F_2}$
Disj	$\frac{I \models F_1 \vee F_2}{I \models F_1 \mid I \models F_2}$	$\frac{I \not\models F_1 \vee F_2}{I \not\models F_1 \quad I \not\models F_2}$
Impl	$\frac{I \models F_1 \rightarrow F_2}{I \not\models F_1 \mid I \models F_2}$	$\frac{I \not\models F_1 \rightarrow F_2}{I \models F_1 \quad I \not\models F_2}$
Contr	$\frac{I \models F \quad I \not\models F}{I \models \perp}$	never (by definition)

The notation $A \mid B$ means “either A or B (or both)”.

Example 1.1. We want to show that the following formula is valid.

$$F \triangleq (P \wedge Q) \rightarrow (P \vee \neg Q)$$

We proceed via proof by contradiction, namely $I \not\models F$

$$\frac{\frac{I \models P \wedge Q}{I \models P \quad I \models Q} \text{CONJ} \quad \frac{I \not\models P \vee \neg Q}{I \not\models P \quad I \not\models \neg Q} \text{DISJ}}{I \not\models (P \wedge Q) \rightarrow (P \vee \neg Q)} \text{IMPL}$$

Since our conclusion has both $I \models P$ and $I \not\models P$ we can note this is a contradiction, and hence F is valid.

2 First-Order Logic

2.1 Semantics

Definition 2.1 (Scope). The *scope* of a quantifier (\forall or \exists) is the formula that immediately follows it. For example, in $\forall x.P(x) \rightarrow Q(x)$ the scope of $\forall x$ is $P(x) \rightarrow Q(x)$. Generally we say for a formula $\forall x.F(x)$ or $\exists x.F(x)$ that the scope of the quantifier is $F(x)$.

- The variable x is *bound* in $F(x)$.
- Any other occurrence of x outside the scope of the quantifier is *free*.
 - A *closed* formula has no free variables.
 - An *open* formula has at least one free variable.

This mirrors lambda calculus in which given a lambda abstraction $\lambda x.M$, the variable x is bound in M and any other occurrence of x outside the scope of the lambda is free.

Definition 2.2 (Domain). The *domain* (or universe) U_I of an interpretation I is a non-empty set of objects (e.g. people, numbers, etc.).

Definition 2.3 (Domain Cardinality). The *cardinality* of a domain U_I is the number of elements in U_I , denoted $|U_I|$. Domains can be finite or infinite, and all are non-empty.

Definition 2.4 (Assignment). An *assignment* α_I or σ of an interpretation I can be classified into 3 types:

- (variable symbols) $x \mapsto x_I \in U_I$
- (n -ary function symbols) $f(t_1, \dots, t_n) \mapsto f_I : U_I^n \rightarrow U_I$
- (n -ary predicate symbols) $p(t_1, \dots, t_n) \mapsto p_I : U_I^n \rightarrow \{\text{true}, \text{false}\}$

Constants are treated as 0-ary function symbols and propositional variables as 0-ary predicate symbols. The lectures denote an assignment of a symbol (variable/function/predicate) x as

$$\sigma[x \mapsto v]$$

which expresses the assignment that agrees with σ to all variables except that x is mapped to v .

Example 2.1 (Assignment). Let $U_I = \{a, b, c\}$ be a domain of people. An assignment σ could be:

- $x \mapsto a$
- $y \mapsto b$
- $f(x) \mapsto \text{"the mother of } x\text{"}$
- $p(x, y) \mapsto \text{"}x \text{ is a parent of } y\text{"}$

Then $\sigma[x \mapsto b]$ would be the same as σ except that $x \mapsto b$.

Definition 2.5 (Interpretation). An *interpretation* is a pair $I : (U_I, \sigma)$ where U_I is a domain and σ is an assignment.

Definition 2.6 (Structure). A *structure* is a pair $S : (U_I, I)$ where U_I is a domain and I is an interpretation.

Definition 2.7 (Subformulae). The *subformulae* of a formula F are the formulae that can be obtained by starting from F and repeatedly applying the following rules:

Algorithm 1 Subformulae extraction

```

1: Input: A formula  $F$ 
2: Output: The set of subformulae of  $F$ 
3: fn SUBFORMULAE( $S$ )
4:   match  $S$  with
5:     case  $\neg G$ :
6:        $S \leftarrow S \cup \text{Subformulae}(G)$ 
7:     case  $G_1 (\wedge \mid \vee \mid \rightarrow) G_2$ :
8:        $S \leftarrow S \cup \text{Subformulae}(G_1) \cup \text{Subformulae}(G_2)$ 
9:     case  $\forall x. G_x \mid \exists x. G_x$ :
10:       $S \leftarrow S \cup \text{Subformulae}(G_x)$ 
11:     case atomic formula:
12:       $S \leftarrow S$ 
13:   end
14: end fn
15:  $S \leftarrow \{F\} \cup \text{Subformulae}(F)$ 

```

Rule	$I \models \cdot$	$I \not\models \cdot$
All	$\frac{S, \sigma \models \forall x. F(x)}{\forall c \in U : S, \sigma[x \mapsto c] \models F(c)}$	$\frac{S, \sigma \not\models \forall x. F(x)}{\exists c \in U : S, \sigma[x \mapsto c] \not\models F(c)}$
Ex	$\frac{S, \sigma \models \exists x. F(x)}{\exists c \in U : S, \sigma[x \mapsto c] \models F(c)}$	$\frac{S, \sigma \not\models \exists x. F(x)}{\forall c \in U : S, \sigma[x \mapsto c] \not\models F(c)}$
Contr	$\frac{S, \sigma \models p(s_1, \dots, s_n) \quad S, \sigma \not\models p(s_1, \dots, s_n)}{S, \sigma \models \perp}$	never (by definition)

3 First-Order Theory

Definition 3.1 (Signature Σ). A *signature* Σ is a set of constant, function and predicate symbols.

Definition 3.2 (Axioms A). A set of *axioms* A is a set of closed formulae in which only symbols from the signature Σ are used. The axioms are what provide meaning to the symbols in the signature.

Definition 3.3 (First-Order Theory). A *first-order theory* is a pair $T : (\Sigma, A)$ where Σ is a signature and A is a set of axioms.

Definition 3.4 (Σ -Formula). A Σ -*formula* is a formula in which only symbols from the signature Σ are used as well as variables, logical connectives, and quantifiers.

Definition 3.5 (Validity in a Theory). A Σ -*formula* F is *valid in a theory* $T : (\Sigma, A)$ if for every structure $S : (\mathcal{U}_I, I)$ such that $S \models A$ it holds that $S \models F$. We denote this as $T \models F$. In other words F is valid in T if its true in all structures (i.e. interpretations) that satisfy the axioms of T . We can express this as a propositional check as follows for a given theory T_K

$$\text{VALIDINTHEORY}(F, T_K) \triangleq \lambda S \mapsto (\lambda A_K \mapsto S \models A_K \rightarrow S \models F) \rightarrow T \models F : \text{Prop} \quad (1)$$

Note: This is not really formally rigorous but just pedagogically I think a nice way of expressing the idea of what constitutes validity in a theory.

4 Congruence

Definition 4.1 (Congruence Relation). In the most general sense a *congruence relation* is a relation R on a given algebraic structure - such as in our case the domain of an interpretation \mathcal{U}_I - if for a given n -ary operation μ (e.g predicate or function symbol) the following condition holds:

$$a_1 R a_2 \wedge \dots \wedge a_n R b_n \implies \mu(a_1, \dots, a_n) R \mu(b_1, \dots, b_n)$$

Within the context of first-order logic we equivalently say given a formula F_1 and F_2 then replacing a subformula F_1 with F_2 within a larger formula F preserves truth.

$$I \models F_1 \leftrightarrow F_2 \implies I \models F[F_1 \mapsto F_2] \Leftrightarrow \frac{I \models F_1 \leftrightarrow F_2}{I \models F[F_1] \leftrightarrow F[F_2]}$$

More generally we can say given n pairs of formulae $F_1, F'_1, \dots, F_n, F'_n$ then replacing each F_i with F'_i within a larger formula F preserves truth.

$$\frac{I \models F_1 \leftrightarrow F'_1 \quad \dots \quad I \models F_n \leftrightarrow F'_n}{I \models F[F_1 \mapsto F'_1, \dots, F_n \mapsto F'_n]}$$

Definition 4.2 (Predicate Congruence). Predicate congruence also known as *Leibniz's Law* or more straightforwardly *Substitution for formulas* states that if two terms t_1 and t_2 are equal then any predicate p that holds for t_1 also holds for t_2 . Formally:

$$\text{PREDCONG}(p) \triangleq t = t' \rightarrow (p(\dots, t, \dots) \leftrightarrow p(\dots, t', \dots)) : \text{Prop} \quad (2)$$

Alternatively we can also use the same notation as for general congruence to express predicate congruence more generally

$$\frac{I \models t_1 = t'_1 \wedge \dots \wedge t_n = t'_n}{I \models p(t_1, \dots, t_n) \leftrightarrow p(t'_1, \dots, t'_n)}$$

Definition 4.3 (Function Congruence). Function congruence is derived as a special case of predicate congruence. We start by defining a formula

$$\text{FUNEQUALS}(t) \triangleq (f(\dots, t, \dots) = f(\dots, t', \dots)) : \text{Prop} \quad (3)$$

We substitute p in equation ?? with $\text{FUNEQUALS}(t')$ to get

$$t = t' \rightarrow (f(\dots, t, \dots) = f(\dots, t, \dots) \rightarrow f(\dots, t, \dots) = f(\dots, t', \dots))$$

We simplify the first implication by noting that $f(\dots, t, \dots) = f(\dots, t, \dots)$ is always true and hence we can remove it to get the definition of function congruence.

$$\text{FUNCONG}(f) \triangleq t = t' \rightarrow (f(\dots, t, \dots) = f(\dots, t', \dots)) : \text{Prop} \quad (4)$$

Again we can also use the same notation as for general congruence to express function congruence as an inference rule

$$\frac{I \models t_1 = t'_1 \wedge \dots \wedge t_n = t'_n}{I \models f(t_1, \dots, t_n) = f(t'_1, \dots, t'_n)}$$

Definition 4.4 (Left / Right Congruence). Left or Right congruence represents a special case of function congruence where the function is a binary operator (e.g. $+$, \times , etc.) and we only replace one of the two arguments. In the most general sense we define some arbitrary binary operator \oplus and then define left and right congruence as follows:

$$\text{LEFTCONG}(\oplus) \triangleq t = t' \rightarrow (t \oplus s = t' \oplus s) : \text{Prop} \quad (5)$$

$$\text{RIGHTCONG}(\oplus) \triangleq s = s' \rightarrow (t \oplus s = t \oplus s') : \text{Prop} \quad (6)$$

Example 4.1 (Small-step operational semantics). *Operational semantics* is just a fancy term for describing how a program executes, in other words the operational semantics of a language describe an idealized interpreter for that language. There are two categories of operational semantics - *big-step* and *small-step*. Big-step semantics are judgements in the form

$$(S, s) \rightarrow s' \equiv \text{Starting in state } s \text{ and executing } S \text{ may terminate in state } s'$$

Small-step semantics are judgements in the form

$$(S, s) \rightarrow (S', s')$$

the conceptual difference is that big-step semantics describe the overall effect of executing a program whereas small-step semantics describe the individual steps taken to execute a program thus giving us a more fine-grained view we can talk about the execution of intermediate states.

A place where Small-step semantics and congruence come together is particularly in the context of *Call by Value* (CBV) evaluation strategy. CBV semantics state that

1. *Right-congruence* : Reduce function expressions until they are values i.e. callable lambdas.

$$\frac{e_1 \rightarrow e'_1}{e_1 e_2 \rightarrow e'_1 e_2} \text{CBV-FUN} \quad (7)$$

2. *Left-congruence* : Function arguments must be fully evaluated before being passed to callable lambdas.

$$\frac{e_1 \rightarrow e'_1}{v e_1 \rightarrow v e'_1} \text{CBV-ARG} \quad (8)$$

3. Function application is only defined when the function is a callable lambda and all arguments are values.

$$\frac{v : \text{value}}{(\lambda x. e) v \rightarrow e[x \mapsto v]} \text{CBV-SUBS} \quad (9)$$

For example consider the following expression

$$(\lambda x. x + 1) (1 + 2)$$

We can evaluate this expression step-by-step using the CBV small-step semantics defined above.

$$\frac{1 + 2 \rightarrow 3}{(\lambda x. x + 1) (1 + 2) \rightarrow (\lambda x. x + 1) 3} \text{CBV-ARG} \quad \frac{3 : \text{value}}{(\lambda x. x + 1) 3 \rightarrow 3 + 1} \text{CBV-SUBS} \quad \frac{3 + 1 \rightarrow 4}{(\lambda x. x + 1) 3 \rightarrow 4} \text{CBV-FUN}$$

Note that we could not have applied the substitution rule (equation ??) first because the argument $1 + 2$ is not a value. We had to first reduce it to a value 3 using the right-congruence rule (equation ??) before we could apply the substitution rule.

5 Equality

5.1 Syntax

Definition 5.1 (Equality Signature). The theory of equality T_E has the *signature* Σ_E defined as follows

$$\Sigma_E : \{=, s\}$$

Where

- $=$ is a binary predicate symbol
- s represents any constant, function or predicate symbol

5.2 Axioms of Equality

The axioms of equality are as follows:

$\text{REFL}(x) \triangleq (x = x)$	(reflexivity)
$\text{SYMM}(x, y) \triangleq (x = y) \rightarrow (y = x)$	(symmetry)
$\text{TRANS}(x, y, z) \triangleq (x = y \wedge y = z) \rightarrow (x = z)$	(transitivity)
$\text{PREDCONG}(p)$	(predicate congruence)
$\text{FUNCONG}(f)$	(function congruence)

6 Peano Arithmetic

6.1 Syntax

Definition 6.1 (PA Signature). The theory of PA has the *signature* Σ_{PA} defined as follows

$$\Sigma_{PA} : \{0, 1, +, \times, =\}$$

Where

- 0 and 1 are constant symbols (0-ary function symbols)
- $+$ and \times are binary function symbols
- $=$ is a binary predicate symbol

6.2 Axioms of PA

The axioms of PA are as follows:

$\forall x. \neg(0 = x + 1) : 0 = \text{MIN}(\mathbb{N})$	(zero)
$\forall x. x + 0 = x$	(plus zero)
$\forall x. \forall y. x + (y + 1) = (x + y) + 1$	(plus successor)
$\forall x. x \times 0 = 0$	(times zero)
$\forall x. \forall y. x \times (y + 1) = (x \times y) + x$	(times successor)
$\forall x. \forall y. (x = y) \rightarrow (x + 1 = y + 1)$	(equality)
$(F(0) \wedge (\forall x. F(x) \rightarrow F(x + 1))) \rightarrow (\forall x. F(x))$	(induction)

7 Presburger Arithmetic

7.1 Syntax

Definition 7.1 (Presburger Signature). The theory of Presburger arithmetic has the *signature* Σ_{Pres} defined as follows

$$\Sigma_{Pres} : \{0, 1, +, =\}$$

Where

- 0 and 1 are constant symbols (0-ary function symbols)
- + is a binary function symbol
- = is a binary predicate symbol

7.2 Axioms of Presburger Arithmetic

The axioms of Presburger arithmetic are as follows:

$$\begin{aligned}
&\forall x. \neg(0 = x + 1) : 0 = \text{MIN}(\mathbb{N}) && (\text{zero}) \\
&\forall x. x + 0 = x && (\text{plus zero}) \\
&\forall x. \forall y. x + (y + 1) = (x + y) + 1 && (\text{plus successor}) \\
&\forall x. \forall y. (x = y) \rightarrow (x + 1 = y + 1) && (\text{equality}) \\
&(F(0) \wedge (\forall x. F(x) \rightarrow F(x + 1))) \rightarrow (\forall x. F(x)) && (\text{induction})
\end{aligned}$$

8 Theory of Arrays

8.1 Syntax

Definition 8.1 (Array Signature). The theory of arrays has the *signature* Σ_{Arrays} defined as follows

$$\Sigma_A : \{ _ [_], \langle _ \triangleleft _ \rangle, = \}$$

Where

- $_ [_]$ is a binary function symbol equivalent to the function $\text{read}(a, i)$ which returns the element at index i of array a .
- $\langle _ \triangleleft _ \rangle$ is a ternary function symbol equivalent to the function $\text{write}(a, i, v)$ which returns a new array that is the same as array a except that index i now contains value v .
- $=$ is a binary predicate symbol.

8.2 Axioms of Arrays

The axioms of the theory of arrays are as follows:

$$\begin{aligned}
&\forall a. \forall i. \forall v. (a \langle i \triangleleft v \rangle)[i] = v && (\text{read-over-write}) \\
&\forall a. \forall i. \forall j. \forall v. (i \neq j) \rightarrow (a \langle i \triangleleft v \rangle)[j] = a[j] && (\text{read-over-write (different index)}) \\
&\forall a. \forall b. (\forall i. a[i] = b[i]) \rightarrow (a = b) && (\text{extensionality})
\end{aligned}$$